Otway-Rees: implemented msg1 interception attack
Attack works similar to msg2 interception but the attacker intercepts earlier
and does not involve the responder in the conversation at all. Hence, we do not
even get mutual auth. in this case.

otway-rees/OYRS.Debug.fst
@@ -38,6 +38,29 @@ let benign_attacker () =
   let msg4_idx = responder_send_msg_4 b msg3_idx b_si in
   initiator_recv_msg_4 a msg4_idx a_si
 
+val intercept_msg_1_attacker:
+  unit ->
+  LCrypto unit (pki oyrs_preds)
+  (requires fun _ -> True)
+  (ensures fun _ _ _ -> True)
+
+let intercept_msg_1_attacker () =
+  let a:principal = "initiator" in
+  let b:principal = "responder" in
+  let srv:principal = "server" in
+
+  let ((|t_as,us_as,k_as|), a_si) = initiator_init a srv b in
+  let ((|t_bs,us_bs,k_bs|), b_si) = responder_init b srv in
+  install_sk_at_auth_server #t_as #us_as srv a k_as;
+  install_sk_at_auth_server #t_bs #us_bs srv b k_bs;
+
+  let msg1_idx = initiator_send_msg_1 a a_si in
+  let (msg4_idx, conv_key) = attacker_intercept_msg_1 b a msg1_idx in
+  initiator_recv_msg_4 a msg4_idx a_si;
+
+  // TODO: no mutual authentication either -> proof needed
+  attacker_knows_conv_key_stored_in_initiator_or_responder_state a a_si conv_key
+
 val intercept_msg_2_attacker:
   unit ->
   LCrypto unit (pki oyrs_preds)
@@ -61,6 +84,7 @@ let intercept_msg_2_attacker () =
   let msg4_idx = responder_send_msg_4 b msg3_idx b_si in
   initiator_recv_msg_4 a msg4_idx a_si;
 
+  // TODO: at least we should get mutual authentication here -> proof needed
   attacker_knows_conv_key_stored_in_initiator_or_responder_state a a_si conv_key;
   attacker_knows_conv_key_stored_in_initiator_or_responder_state b b_si conv_key
 
@@ -69,6 +93,13 @@ let benign () : LCrypto unit (pki oyrs_preds)
 = print_string "start\n";
   let t0 = get() in
   let x = benign_attacker () in
+  print_trace ()
+
+let intercept_msg_1 () : LCrypto unit (pki oyrs_preds)
+  (requires (fun _ -> True)) (ensures (fun _ _ _ -> True))
+= print_string "start\n";
+  let t0 = get() in
+  let x = intercept_msg_1_attacker () in
   print_trace ()
 
 let intercept_msg_2 () : LCrypto unit (pki oyrs_preds)
@@ -90,6 +121,13 @@ let main =
   | Error s -> IO.print_string ("ERROR: "^s^"\n")
   | Success _ -> IO.print_string "PROTOCOL RUN: Successful execution of Otway-Rees protocol.\n");
   IO.print_string "Finished Benign Attacker:\n";
+  IO.print_string "Starting Intercept Msg1 Attacker:\n";
+  assume(valid_trace (pki oyrs_preds) t0);
+  let r,t1 = (reify (intercept_msg_1 ()) t0) in
+  (match r with
+  | Error s -> IO.print_string ("ERROR: "^s^"\n")
+  | Success _ -> IO.print_string "PROTOCOL RUN: Successful execution of Otway-Rees protocol.\n");
+  IO.print_string "Finished Intercept Msg1 Attacker:\n";
   IO.print_string "Starting Intercept Msg2 Attacker:\n";
   assume(valid_trace (pki oyrs_preds) t0);
   let r,t1 = (reify (intercept_msg_2 ()) t0) in
